update single tree - multi tree proof for sign & verify

proof/spec/XMSS_vs_XMSS_MT.ec
@@ -36,6 +36,28 @@ while (#pre).
 - auto.
 qed.
 
+pred eq_auth_path (a : XMSS_Types.AuthPath.auth_path) (a_mt : auth_path)  = 
+    val a_mt = val a.
+
+equiv root_from_sig_equiv : 
+    XMSS_TreeHash.RootFromSig.rootFromSig ~ XMSS_MT_TreeHash.RootFromSig.rootFromSig :
+    ={idx_sig, sig_ots, M, _seed, address} /\
+    eq_auth_path auth{1} auth{2}
+    ==> 
+    ={res}.
+proof.
+proc => /=.
+seq 2 2 : #pre; 1:auto.
+seq 1 1 : (#pre /\ ={pk_ots}); first by call (: ={arg} ==> ={res}); [sim | auto].
+seq 2 2 : #pre; 1:auto.
+seq 1 1 : (#pre /\ ={nodes0}); first by call (: ={arg} ==> ={res}); [sim | auto].
+seq 3 3 : (#pre /\ ={k}); 1:auto.
+while (#pre); auto.
+seq 1 1 : #pre; 1:auto.
+if; [auto | |]; (call (: ={arg} ==> ={res}); [sim |]; by auto => /> &1 &2; rewrite /eq_auth_path => -> ??).
+qed.
+
+
 equiv keygen : 
   XMSS_PRF.kg ~ XMSS_MT_PRF.kg : 
   XMSS_Params.impl_oid = XMSS_MT_Params.impl_oid /\ d = 1 
@@ -49,17 +71,26 @@ seq 6 6 : (#pre /\ ={pub_seed, sk_seed, address, sk_seed, sk_prf, pub_seed}).
 call (treehash_equiv); auto => /> /#.
 qed.
 
-abbrev eqsig(sig : XMSS_Types.sig_t, sigmt : XMSS_MT_Types.sig_t) : bool =
-   sig.`sig_idx = sigmt.`sig_idx /\
-   sig.`r = sigmt.`r /\
-   [sig.`r_sig] = sigmt.`r_sigs.
+pred eq_r_sigs (x : wots_signature * XMSS_Types.AuthPath.auth_path)
+               (y : (wots_signature * auth_path) list) = 
+               size y = 1 /\ 
+               x.`1 = (nth witness y 0).`1 /\ 
+               eq_auth_path x.`2 (nth witness y 0).`2.
+
+pred eqsig(sig : XMSS_Types.sig_t, sigmt : XMSS_MT_Types.sig_t) =
+  sig.`sig_idx = sigmt.`sig_idx /\
+  sig.`r = sigmt.`r /\  
+  eq_r_sigs (sig.`r_sig) (sigmt.`r_sigs).
+
 
 equiv sign : XMSS_PRF.sign ~ XMSS_MT_PRF.sign : 
     XMSS_Params.impl_oid = XMSS_MT_Params.impl_oid /\  
     d=1 /\ 
     h < 32 /\ 0 < to_uint sk{2}.`idx < 2^h - 1 /\ 
-    arg{1}.`1 = arg{2}.`1 /\ arg{1}.`2 = arg{2}.`2 ==> 
-     eqsig res{1}.`1 res{2}.`1 /\ res{1}.`2 = res{2}.`2. 
+    arg{1}.`1 = arg{2}.`1 /\ 
+    arg{1}.`2 = arg{2}.`2 
+    ==> 
+    eqsig res{1}.`1 res{2}.`1 /\ res{1}.`2 = res{2}.`2. 
 proof. 
 proc => /=. 
 rcondf {2} 18.
@@ -67,26 +98,29 @@ rcondf {2} 18.
   wp;call(:true);1:by trivial.
   wp;call(:true);1:by trivial.
   by auto => /> /#.
-
-wp => /=. 
-call(: d=1 /\ ={arg} /\ 0 < to_uint idx{1} /\ to_uint idx{2} < 2 ^ h - 1 ==> ={res}).
-+ proc. 
-  call(: d=1  /\ ={arg} ==> ={res}).
-  + by proc => /=; sim. 
-  wp => /=. 
-  call(: d=1 /\ ={arg} /\ 0 < to_uint idx{1} /\ to_uint idx{2} < 2 ^ h - 1 ==> ={res}).
-  +  proc => /=. 
-     while (#post /\ d = 1 /\ ={address,authentication_path, pub_seed,sk_seed,t,j,idx} /\ 0 <= j{1} <= h /\
-       0 < to_uint idx{1} /\ to_uint idx{2} < 2 ^ h - 1). 
-     + auto => />; conseq (:  ={authentication_path, j,t,address});1:smt().
-     call(:d=1); 1: by conseq />;sim;auto => /> /#.
-     by auto => />.
-   by auto => />; 1: by smt(ge0_h).
-by auto => />.
-
-wp;call(:true); 1: by sim.
-
-
+wp. conseq />.
+call(: 
+  XMSS_Params.impl_oid = XMSS_MT_Params.impl_oid /\ 
+  d = 1 /\ ={arg} /\ 0 < to_uint idx{1} /\ to_uint idx{2} < 2 ^ h - 1 
+  ==> 
+  eq_auth_path res{1}.`2 res{2}.`2 /\ res{1}.`1 = res{2}.`1
+).
++ proc => /=.
+  call (: XMSS_Params.impl_oid = XMSS_MT_Params.impl_oid /\  ={arg} ==> ={res}); 1:sim.
+  wp; conseq />.
+  inline {1} 3; inline {2} 3.
+  wp. 
+  seq 9 9 : (
+    #pre /\ 
+    ={sk_seed, pub_seed, pub_seed0, sk_seed0, idx0, address0, j, t, authentication_path} /\
+    size authentication_path{1} = h /\ 
+    size authentication_path{2} =  h %/ d
+  ); first by auto => /> &2 ?-> /= ??; rewrite !size_nseq; smt(ge0_h).
+  while (#pre); auto => />.
+     - call (treehash_equiv); auto => /> *; split => //; rewrite ?size_put /#. 
+     - move => &2 d_val *; split => [/# |]. 
+       by move => authpathR ?????; rewrite /eq_auth_path !insubdK // /P.
+wp ; call(: true); 1: by sim.
 auto => /> &1 ? -> /= *; do split. 
 + rewrite and_mod;1:smt(ge0_h).
   by rewrite modz_small /=; smt(). 
@@ -96,35 +130,33 @@ auto => /> &1 ? -> /= *; do split.
   rewrite !initiE 1:/# /=.
   rewrite !get_setE 1..3:/#.
   by rewrite initiE 1:/# /=.
-
 + rewrite and_mod;1:smt(ge0_h).
   by rewrite modz_small /=; smt().
-
 qed.
 
 equiv verify : XMSS_PRF.verify ~ XMSS_MT_PRF.verify : 
-    d=1 /\ 
+    d = 1 /\ 
     h < 32 /\ 0 < to_uint s{2}.`sig_idx < 2^h - 1 /\ 
-    arg{1}.`1 = arg{2}.`1 /\ arg{1}.`2 = arg{2}.`2 /\ eqsig arg{1}.`3 arg{2}.`3 ==> ={res}.
-proc.
+    arg{1}.`1 = arg{2}.`1 /\ arg{1}.`2 = arg{2}.`2 /\ eqsig arg{1}.`3 arg{2}.`3 
+    ==> 
+    ={res}.
+proc => /=.
 rcondf {2} 16.
 + move => ?.
   wp;call(:true);1:by trivial.
   by auto => /> /#.
-wp;call(: true); 1: by sim.
-auto => /> &1 &2 -> /=.
-move => /> H H0 H1 H2 H3 H4; do split.
-+ rewrite W32.and_mod /=;1:smt(ge0_h).
-  by rewrite modz_small /=; 1:smt().
-+ rewrite -H4 /=;by smt().
-+ rewrite -H4 /=;by smt().
-+ by smt().
-
-+ rewrite to_uint_shr;1:smt(ge0_h).
-  rewrite /zero_address /set_tree_addr /set_layer_addr /=.
-  have -> : (to_uint s{2}.`sig_idx %/ 2 ^ h) = 0 by smt().
+wp => /=. 
+call root_from_sig_equiv.
+conseq />; 1:smt().
+wp.
+auto => /> &1 &2 -> /= *; do split. 
++ rewrite and_mod;1:smt(ge0_h).
+  by rewrite modz_small /=; smt(). 
++ do congr. rewrite /zero_address /set_tree_addr /set_layer_addr to_uint_shr /=; 1: by smt(ge0_h). 
   apply tP => i ib.
   rewrite !initiE 1:/# /=.
   rewrite !get_setE 1..3:/#.
-  by rewrite initiE 1:/# /=.
+  rewrite (: (to_uint s{2}.`sig_idx %/ 2 ^ h) = 0) 1:/# /=. 
+  case (i = 1) => //?; case (i = 2) => //?; case (i = 0) => //?.
+  by rewrite initiE /=.
 qed.
